theories/Functional/Fun.v
@@ -1,11 +1,16 @@
-Require Import List.
-Require Import Monad.
-Require Import Monad.Folds.
 Require Import Coq.Program.Syntax.
+Require Import List.
+Require Import String.
+Open Scope string_scope.
+
+Require Import Monad.
+Import MonadNotationX.
+Require Import Monad.Folds.
 Require Import Decidables.Decidable.
+Require Import Injection.
 
 Set Implicit Arguments.
-Set Strict Implicit.
+Set Maximal Implicit Insertion.
 
 Module FunNotation.
 
@@ -16,12 +21,13 @@ Module FunNotation.
     (at level 0, only parsing).
 
 End FunNotation.
+Import FunNotation.
 
 Definition compose A B C (g:B -> C) (f:A -> B) (x:A) : C := g (f x).
 
 Definition uncurry A B C (f:A -> B -> C) (x:A * B) : C := let (a,b) := x in f a b.
 
-Definition const {A B} (x:B) : A -> B := fun _ => x.
+Definition const A B (x:B) : A -> B := fun _ => x.
 
 Fixpoint zip A B (xs:list A) (ys:list B) : list (A * B) :=
   match xs, ys with
@@ -31,53 +37,97 @@ Fixpoint zip A B (xs:list A) (ys:list B) : list (A * B) :=
   end
 .
 
-Definition lfst {m} {mMonad:Monad m} {mZero:Zero m} {A} (l:list A) : m A :=
-  match l with
-  | [] => zero
-  | x::_ => ret x
-  end
-.
-
 Definition forEach A B (xs:list A) (f:A -> B) : list B := map f xs.
-
-Definition forEachM {m} {M:Monad m} {A B} (xs:list A) (f:A -> m B) : m (list B) :=
-  mapM f xs.
 
 Section MonadFixDefs.
   Context {m} {mFix:MonadFix m}.
 
-  Definition mfix2 {A B C}
-    (ff:(A -> B -> m C) -> (A -> B -> m C)) (a:A) (b:B) : m C :=
-      let ff' fabp (abp:A*B) :=
-        let (a,b) := abp in
-        let fab a b := fabp (a,b) in
-        ff fab a b
-      in
-      mfix ff' (a,b)
-  .
-
-  Definition mfix3 {A B C D}
-    (ff:(A -> B -> C -> m D) -> (A -> B -> C -> m D))
-    (a:A) (b:B) (c:C) : m D :=
-      let ff' fabcp (abcp:A*B*C) :=
-        let (abp,c) := abcp in
-        let (a,b) := abp in
-        let fabc a b c := fabcp (a,b,c) in
-        ff fabc a b c
-      in
-      mfix ff' (a,b,c)
-  .
 End MonadFixDefs.
 
+Definition lsingleton {A} (x:A) : list A := [x].
+
+Definition firstf {A B C} (f:A->C) (xy:A*B) : C*B :=
+let (x,y) := xy in (f x, y).
+
+Definition secondf {A B C} (f:B->C) (xy:A*B) : A*C :=
+let (x,y) := xy in (x, f y).
+
 Fixpoint update {K V} {kRealDec:RelDec (@eq K)} x v l : list (K * V) :=
-  match l with
-  | [] => [(x,v)]
-  | (y,w)::l' => if eq_dec x y then (x,v)::l' else (y,w)::update x v l'
-  end
-.
+match l with
+| [] => [(x,v)]
+| (y,w)::l' => if eq_dec x y then (x,v)::l' else (y,w)::update x v l'
+end.
 
 Definition updateMany {K V} {kRealDec:RelDec (@eq K)}
   (ups:list (K * V)) (init:list (K * V)) : list (K * V) :=
     fold_right (uncurry update) init ups.
 
-Definition lsingleton {A} (x:A) : list A := [x].
+
+Section monad.
+  Context {m} {mMonad:Monad m}.
+
+  Definition forEachM A {B} (xs:list A) (f:A -> m B) : m (list B) := mapM f xs.
+
+  Definition firstfM {A B C} (fM:A -> m C) (xy:A*B) : m (C*B) :=
+  let (x,y) := xy in x' <- fM x ;; ret (x', y)
+  .
+
+  Definition secondfM {A B C} (fM:B -> m C) (xy:A*B) : m (A*C) :=
+  let (x,y) := xy in y' <- fM y ;; ret (x, y')
+  .
+
+End monad.
+
+Section monadFix.
+  Context {m} {mMonad:Monad m} {mFix:MonadFix m}.
+
+  Definition mfix2 A B C
+    (ff:(A -> B -> m C) -> (A -> B -> m C)) (a:A) (b:B) : m C :=
+  let ff' fabp (abp:A*B) :=
+    let (a,b) := abp in
+    let fab a b := fabp (a,b) in
+    ff fab a b
+  in
+  mfix ff' (a,b)
+  .
+
+  Definition mfix3 A B C D
+    (ff:(A -> B -> C -> m D) -> (A -> B -> C -> m D))
+    (a:A) (b:B) (c:C) : m D :=
+  let ff' fabcp (abcp:A*B*C) :=
+    let (abp,c) := abcp in
+    let (a,b) := abp in
+    let fabc a b c := fabcp (a,b,c) in
+    ff fabc a b c
+  in
+  mfix ff' (a,b,c)
+  .
+
+End monadFix.
+
+Section failure.
+  Context {m} {mMonad:Monad m}.
+  Context {e} {mMonadExc:MonadExc e m} {eInjection:Injection string e}.
+
+  Definition failMsg {A} s : m A := raise (inject s).
+
+  Definition lfirst A (l:list A) : m A :=
+  match l with
+  | [] => failMsg "lfirst of empty list"
+  | x::_ => ret x
+  end.
+
+  Definition lrest A (l:list A) : m (list A) :=
+  match l with
+  | [] => failMsg "lrest of empty list"
+  | _::xs => ret xs
+  end .
+
+  Fixpoint lookup K V {kRealDec:RelDec (@eq K)} (x:K) (l:list (K*V)) : m V :=
+  match l with
+  | [] => failMsg "lookup not in list"
+  | (y,w)::l' => if eq_dec x y then ret w else lookup x l'
+  end.
+
+End failure.
+
